\documentclass[11pt]{article}
\input{../../packages.tex}
\pagestyle{fancy}
\fancyhead[L]{Math 461}
\fancyhead[C]{HW10}
\fancyhead[R]{Lanxiao Bai(lbai5)}
\begin{document}
	\paragraph{6.38}\textbf{Solution:}
		\subparagraph{(a)}
		\[P\{X = i, Y = j\} = \frac{1}{5i}\]
		\subparagraph{(b)}
		\[P\{X = j, Y = i\} = \frac{\sum_{k = i}^5 1 / 5k}{5j} = \frac{\sum_{k = i}^5 1 / k}{j}\]
		\subparagraph{(c)}
		No, $P\{Y\}$ dependent on $P\{X\}$.
	\paragraph{6.40}\textbf{Solution:}
		\subparagraph{(a)}
			\[P\{X = 1\} = p(1, 1) + p(1, 2) = 3/8\]
			\[P\{X = 2\} = p(2, 1) + p(2, 2) = 5/8\]
		\subparagraph{(b)}
			\[P\{X = 1 | Y = 1\} = 1/3 \neq 1/4 = P\{Y = 1\}\]
			$X$ and $Y$ are not independent.
		\subparagraph{(c)}
			\[P\{XY \leq 3\} = 1 - 1/2 = 1/2\]
			\[P\{X + Y > 2\} = 1\]
			\[P\{X / Y > 1\} = 1 / 8\]
	\paragraph{6.41}\textbf{Solution:}
		\subparagraph{(a)}
			\[P\{X = x | Y = y\} = \frac{P\{X = x, Y = y\}}{P\{Y = y\}} \frac{xe^{-x(y+1)}}{\int_0^\infty xe^{-x(y + 1)}dx} = (y + 1)^2 xe^{-x(y + 1)}\]
			\[P\{Y = y | X = x\} = \frac{xe^{-x(y + 1)}}{\int_0^\infty xe^{-x(y + 1)}dy} = xe^{-xy}\]
		\subparagraph{(b)}
			\[P\{Z = XY < a\} = \int_0^\infty \int_0^{a/x}xe^{-x(y + 1)}dydx = 1 - e^{-a}\]
	\paragraph{6.42}\textbf{Solution:}
		\[P\{Y = y | X = x\} = \frac{c(x^2 - y^2)e^{-x}}{\int_{-x}^{x} c(x^2 - y^2)e^{-x}dy} = \frac{3}{4x^3}(x^2 - y^2), -y < x < x\]
	\paragraph{6.48}\textbf{Solution:}
		\subparagraph{(a)}
		\[P\{\min(X_1, \cdots, X_5) \leq a\} = 1 - \prod_{i = 0}^5 P\{X_i > a\} = 1 - e^{-5\lambda a}\]
		\subparagraph{(b)}
		\[P\{\max(X_1, \cdots, X_5) \leq a\} = \prod_{i = 0}^5 P\{X_i > a\} = (1 - e^{-\lambda a})^5\]
\end{document}
