\documentclass[11pt]{article}
\input{../../packages.tex}
\pagestyle{fancy}
\fancyhead[L]{Math 461}
\fancyhead[C]{HW12}
\fancyhead[R]{Lanxiao Bai(lbai5)}
\begin{document}
	\paragraph{7.30}\textbf{Solution:}
	Since $E[X^2] = E[Y^2] = Var(X) + E[X]^2 = \sigma^2 + \mu^2$
		\begin{align}
			&E[(X - Y)^2] = E[X^2 - 2XY + Y^2]\nonumber\\
			&\phantom{E[(X - Y)^2]} = E[X^2] - 2E[XY] + E[Y^2]\nonumber\\
			&\phantom{E[(X - Y)^2]} = E[X^2] - 2E[X][Y] + E[Y^2]\nonumber\\
			&\phantom{E[(X - Y)^2]} = 2\sigma^2\nonumber
		\end{align}
	\paragraph{7.31}\textbf{Solution:}
		\begin{align}
			&Var(\sum_{i = 0}^{10} X) = \sum_{i = 0}^{10} Var(X)\nonumber\\
			&\phantom{Var(\sum_{i = 0}^{10} X)} = \sum_{i = 0}^{10} (E[X^2] - E[X]^2)\nonumber\\
			&\phantom{Var(\sum_{i = 0}^{10} X)} = \sum_{i = 0}^{10} \frac{35}{12} = \frac{175}{6}
		\end{align}
	\paragraph{7.33}\textbf{Solution:}
		\subparagraph{(a)}
			Since $Var(X) = E[X^2] - E[X]^2 \Rightarrow 5 = E[X^2] - 1 \Rightarrow E[X^2] = 6$
			\begin{align}
				&E[(2+X)^2] = E[X^2] + 4E[X] + 4\nonumber\\
				&\phantom{E[(2+X)^2]} = 6 + 4 + 4 = 14
			\end{align}
		\subparagraph{(b)}
			\begin{align}
				&Var(4 + 3X) = 9Var(X) = 45\nonumber
			\end{align}
	\paragraph{7.38}\textbf{Solution:}
		Since $f(x, y) = 2e^{-2x}/x, 0 \leq x < \infty, 0 \leq y \leq x$
		\begin{align}
			&E[XY] = \int_0^{\infty}\int_0^x 2ye^{-2x}dydx = \frac{1}{4} \nonumber\\
			&E[X] = \int_0^{\infty} 2e^{-2x}dydx = \frac{1}{2}\nonumber\\
			&E[Y] = \int_0^{\infty}\int_0^x \frac{2y}{x}e^{-2x}dydx = \frac{1}{4}\nonumber\\
			&Cov(X, Y) = E[XY] - E[X]E[Y]\nonumber\\
			&\phantom{Cov(X, Y)} = \frac{1}{4} - \frac{1}{2}\cdot\frac{1}{4} = \frac{1}{8}
		\end{align}
	\paragraph{7.39}\textbf{Solution:}
		\begin{align}
			&E[Y_n] = E[X_n + X_{n + 1} + X_{n+2}] = \sum_i E[X_{n + i}] = 3\mu\nonumber\\
			&Cov(Y_n, Y_n) = Var(Y_n) = \sum_i Var(X_{n + i}) = 3\sigma^2\nonumber\\
			&Cov(Y_n, Y_{n + 1}) = Cov(X_n + X_{n + 1} + X_{n + 2}, X_{n + 1} + X_{n + 2}, X_{n + 3})\nonumber\\
			&\phantom{Cov(Y_n, Y_{n + 1})} = Cov(X_{n + 1} + X_{n + 2}, X_{n + 1} + X_{n + 2})\nonumber\\
			&\phantom{Cov(Y_n, Y_{n + 1})} = Var(X_{n + 1} + X_{n + 2}) = Var(X_{n + 1}) + Var(X_{n + 2}) = 2\sigma^2\nonumber\\
			&Cov(Y_n, Y_{n + 2}) = Cov(X_n + X_{n + 1} + X_{n + 2}, X_{n + 2} + X_{n + 3}, X_{n + 4})\nonumber\\
			&\phantom{Cov(Y_n, Y_{n + 2})} = Cov(X_{n + 2}, X_{n + 2}) = Var(X_{n + 2}) = \sigma^2\nonumber\\
		\end{align}
		For $j \geq 3$, $Cov(Y_n, Y_{n + j}) = 0$.
	\paragraph{7.41}\textbf{Solution:}
		\[E[X] = 20\cdot 30/100 = 6\]
		\[Var(X) = \frac{20(100 - 20)}{100 - 1}\frac{3}{10}\frac{7}{10} = \frac{112}{33}\]
	\paragraph{7.42}\textbf{Solution:}
		\subparagraph{(a)}
			\[E[\sum_i X_i] = \sum_i E[X_i = 1] = 10 \cdot \frac{2\cdot 10 \cdot 10}{20 \cdot 19} = \frac{100}{19}\]
			\[Var(X_i) = E[X_i^2] - E[X_i]^2 = \frac{10}{19}\]
			\[Cov(X_i, X_j) = E[X_iX_j] - E[X_i]E[X_j] = \frac{10}{19}\cdot\frac{9}{17} - \frac{100}{361} = \frac{90}{6137}\]
			\[Var(\sum_i X_i) = \sum_{i = 1}^{10} Var(X_i)+ 2\sum\sum Cov(X_i, X_j) = \frac{900}{361} + 10\cdot 9 \cdot \frac{10}{6137} = \frac{16200}{6137}\]
		\subparagraph{(b)}
			\[E[\sum_i Y_i] = \sum_i E[Y_i] = 10 \cdot \frac{1}{19} = \frac{10}{19}\]
			\[Var(Y_i) = E[Y_i^2] - E[Y_i]^2 =  \frac{18}{361}\]
			\[Cov(Y_i, Y_j) = E[Y_iY_j] - E[Y_i]E[Y_j] = \frac{8\binom{10}{2}\cdot 16!}{20!} - \frac{1}{361} = \frac{2}{6137} = \frac{10}{6137}\]
			\[Var(\sum_i Y_i) = \sum_{i = 1}^{10} Var(Y_i)+ 2\sum\sum Cov(Y_i, Y_j) = \frac{10\cdot 18}{361} + 90 \cdot \frac{2}{6137} = \frac{3240}{6137}\]
	\paragraph{7.50}\textbf{Solution:}
		Since $f(x, y) = \frac{e^{-x/y}e^{-y}}{y}, 0 < x < \infty, 0 < y < \infty$, then 
		
		\begin{align}
			&f_{X|Y}(x|y) = \frac{f(x, y)}{f_Y(y)}\nonumber\\
			&\phantom{f_{X|Y}(x|y)} = \frac{\frac{e^{-x/y}e^{-y}}{y}}{\int_0^{\infty} \frac{e^{-x/y}e^{-y}}{y}dx}\nonumber\\
			&\phantom{f_{X|Y}(x|y)} = \frac{\frac{e^{-x/y}e^{-y}}{y}}{e^{-y}}\nonumber\\
			&\phantom{f_{X|Y}(x|y)} = \frac{e^{-x/y}}{y}, x > 0\nonumber
		\end{align}
		
		So $E_{X|Y}[X^2 | Y = y] = \int_0^{\infty} \frac{x^2e^{-x/y}}{y}dx = 2y^2$.
	\paragraph{7.51}\textbf{Solution:}
		Since $f(x, y) = \frac{e^{-y}}{y}, 0 < x < y, 0 < y < \infty$, then 
		\begin{align}
			&f_{X|Y}(x|y) = \frac{f(x, y)}{f_Y(y)}\nonumber\\
			&\phantom{f_{X|Y}(x|y)} = \frac{\frac{e^{-y}}{y}}{\int_0^y \frac{e^{-y}}{y} dx}\nonumber\\
			&\phantom{f_{X|Y}(x|y)} = \frac{1}{y}, 0< x < y\nonumber
		\end{align}
		
		So $E_{X|Y}[X^3|Y = y] = \int_0^y \frac{x^3}{y}dx = \frac{y^3}{4}$.
	\paragraph{7.56}\textbf{Solution:}
		Let $Y_i = 1$ if elevator stops at $i$-th floor, so $E[Y_i | X = k] = 1 - (\frac{N - 1}{N})^k$, so
		\[E[\sum_i Y] = \sum_i E[Y_i] = N(1 - (\frac{N - 1}{N})^k)\]
		
		As a result,
		\begin{align}
			&E[Y] = E[E[Y|X]]\nonumber\\
			&\phantom{E[Y]} = E[N(1 - (\frac{N - 1}{N})^k)]\nonumber\\
			&\phantom{E[Y]} = N - NE[(\frac{N - 1}{N})^k)]\nonumber\\
			&\phantom{E[Y]} = N - N\sum_{i = 0}^{\infty} (\frac{N - 1}{N})^k\frac{10k}{k!}e^{-10}\nonumber\\
			&\phantom{E[Y]} = N(1 - e^{-\frac{10}{N}}).\nonumber
		\end{align}
	\paragraph{7.57}\textbf{Solution:}
		\[E[\sum_i Y_i] = E[E[\sum_i Y_i|X]] = 2.5 \cdot 5 = 12.5\]
\end{document}
