\documentclass[11pt]{article}
\input{../../packages.tex}
\pagestyle{fancy}
\fancyhead[L]{Math 461}
\fancyhead[C]{HW9}
\fancyhead[R]{Lanxiao Bai(lbai5)}
\begin{document}
	\paragraph{6.13}\textbf{Solution:}
		\[P(< 5) = \frac{1}{2} \cdot \frac{1}{6} + 1 \cdot \frac{1}{6} = \frac{1}{4}\]
		\[P(man) = \frac{\frac{1}{6}}{\frac{1}{4}} = \frac{2}{3}\]
	\paragraph{6.14}\textbf{Solution:}
		\[P\{|Y - X| < a\} = \frac{2}{L^2}\int_0^L\int_y^{\min(y+a, L)}dxdy = \frac{a}{L}(2 - \frac{a}{L}), 0 < a < L\]
	\paragraph{6.20}\textbf{Solution:}
		\[f_X(x) = xe^{-x}, f_Y(y) = e^{-y}, f(x,y) = xe^{-(x+y)} = f_X(x)f_Y(y)\]
		So $X$ and $Y$ are independent.
		
		\[f_X(x) = 2(1 - x)\]
		\[f_Y(y) = 2y\]
		\[f_X(x)f_Y(y) = 4y(1 - x) \neq f(x, y)\]
		So $X$ and $Y$ are dependent.
	\paragraph{6.21}\textbf{Solution:}
		\subparagraph{(a)}
			\[\iint 24xydxdy = 24\int_0^1 \int_0^{1-y} xydxdy = 1\]
		\subparagraph{(b)}
			\[E[X] = \int_0^1 x\int_0^{1-x} 24xydydx = 2/5\]
		\subparagraph{(c)}
			\[E[Y] = \int^1_0 y\int^{1-y}_0 24xydxdy = 2/5\]
	\paragraph{6.22}\textbf{Solution:}
		\subparagraph{(a)}
			No, $f(x,y)$ does not factor.
		\subparagraph{(b)}
			\[f_X(x) = \int_0^1 (x+y)dy = x + 1/2, 0 < x < 1\]
		\subparagraph{(c)}
			\[P\{X + Y < 1\} = \int_0^1\int_0^{1-x}(x+y)dydx = 1/3\]
	\paragraph{6.23}\textbf{Solution:}
		\subparagraph{(a)}
			\[f_X(x) = \int_0^1 12xy(1-x)dy = 6x(1-x), 0 < x < 1\]
			\[f_Y(y) = \int_0^1 12xy(1-x)dx = 2y, 0 < y < 1\]
			\[f_X(x)f_Y(y) = 12xy(1 - x) = f(x, y)\]
			So $X$ and $Y$ are independent.
		\subparagraph{(b)}
			\[E[X] = \int_0^1 x\int_0^1 12xy(1 - x)dydx = 1/2\]
		\subparagraph{(c)}
			\[E[Y] = \int_0^1 y\int_0^1 12xy(1 - x)dxdy = 2/3\]
		\subparagraph{(d)}
			\[Var(X) = \int_0^1 6x^3(1-x)dx - 1/4  = 1/20\]
		\subparagraph{(e)}
			\[Var(Y) = \int_0^1 2y^3dy - 4/9 = 1/18\]
	\paragraph{6.27}\textbf{Solution:}
			\[P\{a\} = \int_0^{\infty}\int_0^{ay} \lambda_1e^{-\lambda_1x}\lambda_2e^{-\lambda_2x} dxdy = \frac{\lambda_1a}{a\lambda_1 + \lambda_2}\]
			\[P\{X_1 < X_2\} = P\{X_1 / X_2 < 1\} = \frac{\lambda_1}{\lambda_1 + \lambda_2}\]
	\paragraph{6.28}\textbf{Solution:}
		\[f(t) = e^{-x}\]
		\subparagraph{(a)}
			\[P\{MJ\} = \frac{1}{2}e^{-t}\]
		\subparagraph{(b)}
			\[P\{MJ\} = 1 - 3e^{-2}\]
	\paragraph{6.29}\textbf{Solution:}
		\subparagraph{(a)}
			\[P\{X > 5000\} = P\{Z > \frac{5000 - 4400}{\sqrt{2(230)^2}}\} = 0.0326\]
		\subparagraph{(b)}
			\[P\{X > 2000\} = P\{Z > (2000 - 2200)/230\} = 0.8078\]
		
	\paragraph{6.33}\textbf{Solution:}
		\subparagraph{(a)}
			\[p = 1 - e^{-0.2} - 0.2e^{-0.2} - e^{-0.2}(0.2)^2/2!\]
		\subparagraph{(b)}
			\[p = 1 - \sum_{i = 0}^2 e^{-0.2}(0.2)^i/i!\]
\end{document}
